@prefix :        <http://vocab.linkeddata.es/datosabiertos/def/sector-publico/servicio#> .
@prefix dc:      <http://purl.org/dc/elements/1.1/> .
@prefix foaf:    <http://xmlns.com/foaf/0.1/> .
@prefix vann:    <http://purl.org/vocab/vann/> .
@prefix owl2:    <http://www.w3.org/2006/12/owl2#> .
@prefix geonames:  <http://www.geonames.org/ontology#> .
@prefix vcard:   <http://www.w3.org/2006/vcard/ns#> .
@prefix dcterms:  <http://purl.org/dc/terms/> .
@prefix schema:  <http://schema.org/> .
@prefix rdfs:    <http://www.w3.org/2000/01/rdf-schema#> .
@prefix geosparql:  <http://www.opengis.net/ont/geosparql#> .
@prefix esadm:   <http://vocab.linkeddata.es/datosabiertos/def/sector-publico/territorio#> .
@prefix dctype:  <http://purl.org/dc/dcmitype/> .
@prefix dbpedia:  <http://dbpedia.org/ontology/> .
@prefix esproc:  <http://vocab.linkeddata.es/datosabiertos/def/sector-publico/servicio#> .
@prefix xsd:     <http://www.w3.org/2001/XMLSchema#> .
@prefix owl:     <http://www.w3.org/2002/07/owl#> .
@prefix rdf:     <http://www.w3.org/1999/02/22-rdf-syntax-ns#> .
@prefix skos:    <http://www.w3.org/2004/02/skos/core#> .
@prefix cc:      <http://creativecommons.org/ns#> .

esproc:lugarPago
      a       owl:ObjectProperty ;
      rdfs:comment "Lugar de pago del procedimiento, en caso de tener que realizar pago"@es ;
      rdfs:domain esproc:Procedimiento ;
      rdfs:isDefinedBy <http://vocab.linkeddata.es/datosabiertos/def/sector-publico/servicio> ;
      rdfs:label "lugar de pago"@es ;
      rdfs:range esproc:CentroServicio ;
      rdfs:subPropertyOf <http://purl.org/vocab/cpsv#hasChannel> ;
      dcterms:issued "2016-07-28" .

esproc:detalleTramitacionEnLinea
      a       owl:ObjectProperty ;
      rdfs:comment "The detalleTramitacionEnLinea property links an online-based service to the Rule(s) under which it operates."@en ;
      rdfs:domain esproc:ProcedimientoPorEnLinea ;
      rdfs:range esproc:ProcedimientoProceso ;
      rdfs:subPropertyOf esproc:normativa .

esproc:requisitos
      a       owl:DatatypeProperty ;
      rdfs:comment "This property links a PublicService with its requirements (in text format)" ;
      rdfs:domain esproc:Procedimiento ;
      rdfs:range xsd:string ;
      rdfs:subPropertyOf esproc:hasInputTexto .

esproc:normativa
      a       owl:ObjectProperty ;
      rdfs:comment "The normativa property links a Public Service to a Rule"@en ;
      rdfs:domain esproc:Procedimiento ;
      rdfs:subPropertyOf <http://purl.org/vocab/cpsv#follows> .

esproc:pregunta
      a       owl:ObjectProperty ;
      rdfs:comment "This property links a Public Service to the question associated to the service."@en ;
      rdfs:domain
              [ a       owl:Class ;
                owl:unionOf (esproc:Materia esproc:Pregunta)
              ] ;
      rdfs:range esproc:Pregunta ;
      rdfs:subPropertyOf owl:topObjectProperty .

esproc:organo
      a       owl:ObjectProperty ;
      rdfs:comment "To  be completed"@en ;
      rdfs:domain esproc:Procedimiento ;
      rdfs:range esproc:GestorDecisor ;
      rdfs:subPropertyOf <http://purl.org/vocab/cpsv#hasChannel> .

esproc:permiteTramitacionEnLinea
      a       owl:DatatypeProperty ;
      rdfs:domain <http://purl.org/vocab/cpsv#PublicService> ;
      rdfs:range xsd:boolean ;
      rdfs:subPropertyOf esproc:permiteTramitation .

rdfs:comment
      a       owl:AnnotationProperty .

esproc:tipoVia
      a       owl:ObjectProperty ;
      rdfs:comment """Tipo de vía, que será representado mediante la clasificación en SKOS de URI http://vocab.linkeddata.es/datosabiertos/kos/urbanismo-infraestructuras/tipo-via.
Por ejemplo, estas serán las URIs correspondientes a calles y plazas
http://vocab.linkeddata.es/datosabiertos/kos/urbanismo-infraestructuras/tipo-via/CL
http://vocab.linkeddata.es/datosabiertos/kos/urbanismo-infraestructuras/tipo-via/PL"""@es ;
      rdfs:domain esproc:Via ;
      rdfs:isDefinedBy <http://vocab.linkeddata.es/datosabiertos/def/sector-publico/servicio> ;
      rdfs:label "tipo de vía"@es ;
      rdfs:range skos:Concept ;
      dcterms:issued "2014-03-28"^^xsd:dateTime .

esproc:enLineaDocumentacionTexto
      a       owl:DatatypeProperty ;
      rdfs:comment "This property links an online-based Public Service with its inputs/requirements (in string format)."@en ;
      rdfs:domain esproc:ProcedimientoPorEnLinea ;
      rdfs:range xsd:string ;
      rdfs:subPropertyOf esproc:hasInputTexto .

esproc:pago
      a       owl:DatatypeProperty ;
      rdfs:comment "Information about the payment (date, amount, place) for a Public Service"@en ;
      rdfs:domain esproc:Procedimiento ;
      rdfs:range xsd:string .

rdfs:isDefinedBy
      a       owl:AnnotationProperty .

esproc:permiteTramitacionPresencial
      a       owl:DatatypeProperty ;
      rdfs:domain <http://purl.org/vocab/cpsv#PublicService> ;
      rdfs:range xsd:boolean ;
      rdfs:subPropertyOf esproc:permiteTramitation .

esproc:enLineaDocumentacion
      a       owl:ObjectProperty ;
      rdfs:comment "This property links an online-based Public Service with its inputs/requirements."@en ;
      rdfs:domain esproc:ProcedimientoPorEnLinea ;
      rdfs:range esproc:DocumentacionEntrada ;
      rdfs:subPropertyOf <http://purl.org/vocab/cpsv#hasInput> .

esproc:lugarPresentacionTexto
      a       owl:DatatypeProperty ;
      rdfs:comment "The place to present the application for a Public Service (in string format)"@en ;
      rdfs:domain esproc:Procedimiento ;
      rdfs:range xsd:string ;
      rdfs:subPropertyOf esproc:hasChannelTexto .

esproc:claseTerminacion
      a       owl:ObjectProperty ;
      rdfs:comment "To be completed"@en ;
      rdfs:domain esproc:Procedimiento .

esproc:ProcedimientoPorCorreo
      a       owl:Class ;
      rdfs:subClassOf esproc:Procedimiento .

esproc:tipoProcedimiento
      a       owl:ObjectProperty ;
      rdfs:comment "this property links a Public Service with the type of the Public Service."@en ;
      rdfs:domain esproc:Procedimiento ;
      rdfs:range esproc:TipoProcedimiento .

esproc:fechaPresentacionTexto
      a       owl:DatatypeProperty ;
      rdfs:comment "fecha en la que se deben presentar las solicitudes (en formato textual)"@es ;
      rdfs:domain esproc:Procedimiento ;
      rdfs:isDefinedBy <http://vocab.linkeddata.es/datosabiertos/def/sector-publico/servicio> ;
      rdfs:label "fecha de presentación (formato texto)"@es ;
      rdfs:range xsd:string ;
      dcterms:issued "2016-07-28" .

esproc:respuestaAceptada
      a       owl:ObjectProperty ;
      rdfs:comment "Defined as a subproperty of schema:acceptedAnswer, this property links a question (essrvc:Pregunta) with its answer (essrvc:Respuesta)"@en ;
      rdfs:domain esproc:Pregunta ;
      rdfs:range esproc:Respuesta ;
      rdfs:subPropertyOf schema:acceptedAnswer .

esproc:fechaPlazoInicio
      a       owl:DatatypeProperty ;
      rdfs:comment "This property represent the deadline to start a Public Service."@en ;
      rdfs:domain esproc:Procedimiento ;
      rdfs:range xsd:dateTime .

esproc:proporcionadoPor
      a       owl:ObjectProperty ;
      rdfs:comment "this property is the inverse of cpsv:provides."@en ;
      rdfs:domain <http://purl.org/vocab/cpsv#PublicService> ;
      rdfs:range dcterms:Agent .

esproc:dirigidoPor
      a       owl:ObjectProperty ;
      rdfs:comment "This property links a Public Service with an Entity that uses it"@en ;
      rdfs:domain esproc:Procedimiento ;
      rdfs:range esproc:DestinadoProcedimiento ;
      rdfs:subPropertyOf esproc:usadoPor .

esproc:recursoProcede
      a       owl:ObjectProperty ;
      rdfs:comment "To  be completed"@en ;
      rdfs:domain <http://purl.org/vocab/cpsv#PublicService> ;
      rdfs:range esproc:Recurso .

esproc:recursoProcedeTexto
      a       owl:DatatypeProperty ;
      rdfs:comment "to be completed"@en ;
      rdfs:domain esproc:Procedimiento ;
      rdfs:range xsd:string .

esproc:permiteTramitationCorreoPostal
      a       owl:DatatypeProperty ;
      rdfs:domain <http://purl.org/vocab/cpsv#PublicService> ;
      rdfs:range xsd:boolean ;
      rdfs:subPropertyOf esproc:permiteTramitation .

esproc:claseTerminacionTexto
      a       owl:DatatypeProperty ;
      rdfs:comment "to be completed."@en ;
      rdfs:domain esproc:Procedimiento ;
      rdfs:range xsd:string .

esproc:detalleTramitacionTelefono
      a       owl:ObjectProperty ;
      rdfs:comment "The detalleTramitacionEnLinea property links a telephone-based service to the Rule(s) under which it operates."@en ;
      rdfs:domain <http://purl.org/vocab/cpsv#PublicService> ;
      rdfs:range esproc:ProcedimientoProceso ;
      rdfs:subPropertyOf esproc:normativa .

esproc:permiteTramitacionCorreoCertificado
      a       owl:DatatypeProperty ;
      rdfs:domain <http://purl.org/vocab/cpsv#PublicService> ;
      rdfs:range xsd:boolean ;
      rdfs:subPropertyOf esproc:permiteTramitation .

esproc:respuestaTexto
      a       owl:DatatypeProperty ;
      rdfs:comment "the answer of a question in string format" ;
      rdfs:domain esproc:Pregunta ;
      rdfs:range xsd:string .

esproc:materiaDePregunta
      a       owl:ObjectProperty ;
      rdfs:comment "To  be completed"@en ;
      rdfs:domain esproc:Pregunta ;
      rdfs:range esproc:Materia .

esproc:preguntaDeProcedimiento
      a       owl:ObjectProperty ;
      rdfs:domain esproc:Procedimiento ;
      rdfs:range esproc:Pregunta ;
      rdfs:subPropertyOf esproc:pregunta .

esproc:procedimientoDeMateria
      a       owl:ObjectProperty ;
      rdfs:comment "To  be completed"@en ;
      rdfs:domain esproc:Materia ;
      rdfs:range esproc:Procedimiento .

esproc:DestinadoProcedimiento
      a       owl:Class ;
      rdfs:comment "This class represent the target entity of a Public Service."@en ;
      rdfs:subClassOf dcterms:Agent .

esproc:detalleTramitacionPresencialTexto
      a       owl:DatatypeProperty ;
      rdfs:comment "This property links a presencial-based PublicService with the rules that it follows (in text format)."@en ;
      rdfs:domain esproc:ProcedimientoPorPresencial ;
      rdfs:range xsd:string ;
      rdfs:subPropertyOf esproc:followsTexto .

schema:Place
      a       owl:Class .

esproc:Pregunta
      a       owl:Class ;
      rdfs:comment "a subclass of schema:Question"@en ;
      rdfs:subClassOf schema:Question .

<http://www.w3.org/ns/org#Organization>
      a       owl:Class .

esproc:Impreso
      a       owl:Class ;
      rdfs:comment "This class represents Forms to be filled in order to request a Public Servcie"@en ;
      rdfs:subClassOf <http://purl.org/vocab/cpsv#Input> .

esproc:Gestor
      a       owl:Class ;
      rdfs:comment "This class represent an entity that manages a Public Service"@en ;
      rdfs:subClassOf esproc:GestorDecisor .

esproc:otroLugarPresentacion
      a       owl:ObjectProperty ;
      rdfs:comment "This property links a Public Service with the organization to which the application is to be presented."@en ;
      rdfs:domain esproc:Procedimiento ;
      rdfs:range esproc:CentroServicio ;
      rdfs:subPropertyOf <http://purl.org/vocab/cpsv#hasChannel> .

esproc:ProcedimientoPorEnLinea
      a       owl:Class ;
      rdfs:subClassOf esproc:Procedimiento .

schema:CivicStructure
      a       owl:Class .

geonames:R
      a       owl:NamedIndividual , skos:Concept .

[]    rdfs:label "HTML" .

esproc:TipoProcedimiento
      a       owl:Class .

esproc:Materia
      a       owl:Class ;
      rdfs:comment "To  be completed"@en .

esproc:ProcedimientoPorPresencial
      a       owl:Class ;
      rdfs:subClassOf esproc:Procedimiento .

esproc:lugarPagoTexto
      a       owl:DatatypeProperty ;
      rdfs:comment "Lugar donde se realiza el pago del servicio, en caso de que haya que realizar pago (en formato textual)"@es ;
      rdfs:domain esproc:Procedimiento ;
      rdfs:isDefinedBy <http://vocab.linkeddata.es/datosabiertos/def/sector-publico/servicio> ;
      rdfs:label "lugar de pago (formato texto)"@es ;
      rdfs:range xsd:string ;
      rdfs:subPropertyOf esproc:hasChannelTexto ;
      dcterms:issued "2016-07-28" .

esproc:hasInputTexto
      a       owl:DatatypeProperty ;
      rdfs:comment "The inputs for a Public Service (in string format)"@en ;
      rdfs:domain esproc:Procedimiento ;
      rdfs:range xsd:string .

<http://purl.org/vocab/cpsv#hasInput>
      rdfs:domain <http://purl.org/vocab/cpsv#PublicService> .

esproc:correoDocumentacionTexto
      a       owl:DatatypeProperty ;
      rdfs:comment "This property links a postal mail based Public Service with its inputs/requirements (in string format)."@en ;
      rdfs:domain esproc:ProcedimientoPorCorreo ;
      rdfs:subPropertyOf esproc:hasInputTexto .

esproc:MaterialAgrupacion
      a       owl:Class ;
      rdfs:comment "To  be completed"@en .

rdfs:label
      a       owl:AnnotationProperty .

esproc:detalleTramitacionCorreoPostal
      a       owl:ObjectProperty ;
      rdfs:comment "The detalleTramitacionCorreoPostal property links a postal mail based service to the Rule(s) under which it operates."@en ;
      rdfs:domain esproc:ProcedimientoPorCorreo ;
      rdfs:range esproc:ProcedimientoProceso ;
      rdfs:subPropertyOf esproc:normativa .

esproc:Decisor
      a       owl:Class ;
      rdfs:comment "This class represent an entity that makes decision in a Public Service"@en ;
      rdfs:subClassOf esproc:GestorDecisor .

esproc:Procedimiento
      a       owl:Class ;
      rdfs:comment "a subclass of cpsv:PublicService"@en ;
      rdfs:subClassOf <http://purl.org/vocab/cpsv#PublicService> .

esproc:presentar
      a       owl:ObjectProperty ;
      rdfs:comment "The organization in which the application for a Public Service is to be presented."@en ;
      rdfs:domain esproc:Procedimiento ;
      rdfs:range esproc:CentroServicio ;
      rdfs:subPropertyOf <http://purl.org/vocab/cpsv#hasChannel> .

skos:Concept
      a       owl:Class .

esproc:claseIniciacion
      a       owl:ObjectProperty ;
      rdfs:comment "To be completed"@en ;
      rdfs:domain esproc:Procedimiento .

esproc:DocumentacionEntrada
      a       owl:Class ;
      rdfs:comment "DocumentacionEntrada, a subclass of cpsv:Input represents the input of a public service"@en ;
      rdfs:subClassOf <http://purl.org/vocab/cpsv#Input> .

schema:question
      a       owl:ObjectProperty .

esproc:ProcedimientoProceso
      a       owl:Class ;
      rdfs:comment "ProcedimientoProceso, a subclass of Rule, represents a rule that has to be followed by a Procedimiento"@en ;
      rdfs:subClassOf <http://purl.org/vocab/cpsv#Rule> .

esproc:detalleTramitacionCorreoPostalTexto
      a       owl:DatatypeProperty ;
      rdfs:comment "This property links a postal-mail based PublicService with the rules that it follows (in text format)."@en ;
      rdfs:domain esproc:ProcedimientoPorCorreo ;
      rdfs:subPropertyOf esproc:followsTexto .

esproc:fechaRespuestaTexto
      a       owl:DatatypeProperty ;
      rdfs:comment "fecha en la que se deben resolver las solicitudes (en formato textual)"@es ;
      rdfs:domain esproc:Procedimiento ;
      rdfs:isDefinedBy <http://vocab.linkeddata.es/datosabiertos/def/sector-publico/servicio> ;
      rdfs:label "fecha de respuesta (formato texto)"@es ;
      rdfs:range xsd:string ;
      dcterms:issued "2016-07-28" .

esproc:enLineaURL
      a       owl:ObjectProperty ;
      rdfs:comment "This property links a online-based PublicService with its URL"@en ;
      rdfs:domain esproc:Procedimiento ;
      rdfs:subPropertyOf <http://purl.org/vocab/cpsv#hasChannel> .

schema:Question
      a       owl:Class .

esproc:presencialDocumentacion
      a       owl:ObjectProperty ;
      rdfs:comment "This property links a presence-based Public Service with its inputs/requirements."@en ;
      rdfs:domain esproc:ProcedimientoPorPresencial ;
      rdfs:range esproc:DocumentacionEntrada ;
      rdfs:subPropertyOf <http://purl.org/vocab/cpsv#hasInput> .

dcterms:issued
      a       owl:AnnotationProperty .

schema:Answer
      a       owl:Class .

esproc:preguntaDeMateria
      a       owl:ObjectProperty ;
      rdfs:domain esproc:Materia ;
      rdfs:range esproc:Pregunta ;
      rdfs:subPropertyOf esproc:pregunta .

<http://vocab.linkeddata.es/datosabiertos/def/sector-publico/servicio>
      a       owl:Ontology ;
      rdfs:comment """Este vocabulario se utiliza para la descripción de procedimientos administrativos ofrecidos por un ayuntamiento. Reutiliza términos de varios vocabularios, como:
- schema.org
- CPSV (Core Public Service Vocabulary)
- Unidades territoriales en España
Asimismo, se actualizará de acuerdo con la evolución de estos vocabularios (especialmente los que están en pleno desarrollo en el momento de creación de este vocabulario, como el vocabulario sobre unidades territoriales en España).
		"""@es ;
      cc:license <http://creativecommons.org/licenses/by/4.0/> ;
      dc:creator "Freddy Priyatna (Ontology Engineering Group, Universidad Politécnica de Madrid)" , "Víctor Morlán (Ayuntamiento de Zaragoza)" , "Oscar Corcho (Ontology Engineering Group, Universidad Politécnica de Madrid)" ;
      dc:date "2016-07-28"^^xsd:dateTime ;
      dc:identifier "http://vocab.linkeddata.es/datosabiertos/def/sector-publico/servicio"^^xsd:dateTime ;
      dc:rights "Creative Commons Attribution 4.0 International (CC BY 4.0)" ;
      dc:title "Vocabulario para la representación de procedimientos administrativos ofrecidos por un ayuntamiento"@es ;
      dcterms:description """Este vocabulario se utiliza para la descripción de procedimientos administrativos ofrecidos por un ayuntamiento. Reutiliza términos de varios vocabularios, como:
- schema.org
- CPSV (Core Public Service Vocabulary)
- Unidades territoriales en España
Asimismo, se actualizará de acuerdo con la evolución de estos vocabularios (especialmente los que están en pleno desarrollo en el momento de creación de este vocabulario, como el vocabulario sobre unidades territoriales en España)."""@es ;
      dcterms:hasFormat <http://vocab.linkeddata.es/datosabiertos/def/sector-publico/servicio.rdf> , <http://vocab.linkeddata.es/datosabiertos/def/sector-publico/servicio.html> ;
      dcterms:issued "2016-07-28"^^xsd:dateTime ;
      vann:preferredNamespaceUri
              esproc: ;
      owl:imports <http://purl.org/vocab/cpsv> ;
      owl:versionIRI <http://vocab.linkeddata.es/datosabiertos/def/sector-publico/servicio/0.1> .

esproc:permiteTramitacionTelefono
      a       owl:DatatypeProperty ;
      rdfs:domain <http://purl.org/vocab/cpsv#PublicService> ;
      rdfs:range xsd:boolean ;
      rdfs:subPropertyOf esproc:permiteTramitation .

esproc:hasChannelTexto
      a       owl:DatatypeProperty ;
      rdfs:domain esproc:Procedimiento .

esproc:telefonoDocumentacion
      a       owl:ObjectProperty ;
      rdfs:comment "This property links a telephone-based Public Service with its inputs/requirements."@en ;
      rdfs:domain esproc:ProcedimientoPorTelefono ;
      rdfs:range esproc:DocumentacionEntrada ;
      rdfs:subPropertyOf <http://purl.org/vocab/cpsv#hasInput> .

esproc:Normativa
      a       owl:Class ;
      rdfs:comment "Normativa, a subclass of Rule, represents a rule that has to be followed by a PublicService"@en ;
      rdfs:subClassOf <http://purl.org/vocab/cpsv#Rule> .

esproc:detalleTramitacionEnLineaTexto
      a       owl:DatatypeProperty ;
      rdfs:comment "This property links an online-based PublicService with the rules that it follows (in text format)."@en ;
      rdfs:domain esproc:ProcedimientoPorEnLinea ;
      rdfs:range xsd:string ;
      rdfs:subPropertyOf esproc:followsTexto .

esproc:Via
      a       owl:Class .

esproc:fechaRespuesta
      a       owl:DatatypeProperty ;
      rdfs:comment "fecha en la que se deben resolver las solicitudes (en formato fecha/duración)"@es ;
      rdfs:domain esproc:Procedimiento ;
      rdfs:isDefinedBy <http://vocab.linkeddata.es/datosabiertos/def/sector-publico/servicio> ;
      rdfs:label "fecha de respuesta (formato fecha)"@es ;
      rdfs:range xsd:dateTime ;
      dcterms:issued "2016-07-28" .

esproc:lugarPresentacion
      a       owl:ObjectProperty ;
      rdfs:comment "This property links a Public Service with the organization to which the application is to be presented."@en ;
      rdfs:domain esproc:Procedimiento ;
      rdfs:range esproc:CentroServicio ;
      rdfs:subPropertyOf <http://purl.org/vocab/cpsv#hasChannel> .

esproc:GestorDecisor
      a       owl:Class ;
      rdfs:comment "This class represent an entity that makes decision or manages a Public Service"@en ;
      rdfs:subClassOf dcterms:Agent .

esproc:info
      a       owl:ObjectProperty ;
      rdfs:comment "This property links a Public Service with the organization that provide information for the corresponding Public Service."@en ;
      rdfs:domain esproc:Procedimiento ;
      rdfs:range esproc:CentroServicio ;
      rdfs:subPropertyOf <http://purl.org/vocab/cpsv#hasChannel> .

schema:acceptedAnswer
      a       owl:ObjectProperty .

esproc:detalleTramitacionPresencial
      a       owl:ObjectProperty ;
      rdfs:comment "The detalleTramitacionPresencial property links a presence-based service to the Rule(s) under which it operates."@en ;
      rdfs:domain esproc:ProcedimientoPorPresencial ;
      rdfs:range esproc:ProcedimientoProceso ;
      rdfs:subPropertyOf esproc:normativa .

<http://purl.org/vocab/cpsv#hasChannel>
      a       owl:ObjectProperty .

esproc:fechaPlazoFin
      a       owl:DatatypeProperty ;
      rdfs:comment "This property represents the deadline to terminate a public service."@en ;
      rdfs:domain esproc:Procedimiento ;
      rdfs:range xsd:dateTime .

esproc:Respuesta
      a       owl:Class ;
      rdfs:comment "This class represents the answers for a question."@en ;
      rdfs:subClassOf schema:Answer .

owl:topDataProperty
      a       owl:AnnotationProperty ;
      rdfs:domain <http://purl.org/vocab/cpsv#PublicService> .

esproc:claseIniciacionTexto
      a       owl:DatatypeProperty ;
      rdfs:comment "to be completed."@en ;
      rdfs:domain esproc:Procedimiento ;
      rdfs:range xsd:string .

esproc:permiteTramitation
      a       owl:DatatypeProperty ;
      rdfs:comment "we should replace all the subproperties with SKOS"@en ;
      rdfs:domain esproc:Procedimiento ;
      rdfs:range xsd:boolean .

esproc:presencialDocumentacionTexto
      a       owl:DatatypeProperty ;
      rdfs:comment "This property links a presence-based Public Service with its inputs/requirements (in string format)."@en ;
      rdfs:domain esproc:ProcedimientoPorPresencial ;
      rdfs:range xsd:string ;
      rdfs:subPropertyOf esproc:hasInputTexto .

esproc:ProcedimientoPorTelefono
      a       owl:Class ;
      rdfs:subClassOf esproc:Procedimiento .

esproc:fechaPresentacion
      a       owl:DatatypeProperty ;
      rdfs:comment "fecha en la que se deben presentar las solicitudes (en formato fecha)"@es ;
      rdfs:domain esproc:Procedimiento ;
      rdfs:isDefinedBy <http://vocab.linkeddata.es/datosabiertos/def/sector-publico/servicio> ;
      rdfs:label "fecha de presentación (formato fecha)"@es ;
      rdfs:range xsd:dateTime ;
      dcterms:issued "2016-07-28" .

<http://purl.org/vocab/cpsv#provides>
      owl:inverseOf esproc:proporcionadoPor .

esproc:efectoSilencioAdministrativo
      a       owl:DatatypeProperty ;
      rdfs:comment "situation that occurs if there is no response from the entity who is in charge with a Public Service."@en .

[]    rdfs:label "RDF" .

esproc:usadoPor
      a       owl:ObjectProperty ;
      rdfs:domain <http://purl.org/vocab/cpsv#PublicService> ;
      rdfs:label """This property is the inverse of cpsv:uses property.
This property link a PublicService to an Agent via a \"used-by\" relationship."""^^xsd:string ;
      rdfs:range dcterms:Agent .

esproc:correoDocumentacion
      a       owl:ObjectProperty ;
      rdfs:comment "This property links a postal mail based Public Service with its inputs/requirements."@en ;
      rdfs:domain esproc:ProcedimientoPorCorreo ;
      rdfs:range esproc:DocumentacionEntrada ;
      rdfs:subPropertyOf <http://purl.org/vocab/cpsv#hasInput> .

esproc:telefonoDocumentacionTexto
      a       owl:DatatypeProperty ;
      rdfs:comment "This property links a telephone-based Public Service with its inputs/requirements (in string format)."@en ;
      rdfs:domain esproc:ProcedimientoPorTelefono ;
      rdfs:range xsd:string ;
      rdfs:subPropertyOf esproc:hasInputTexto .

esproc:followsTexto
      a       owl:DatatypeProperty ;
      rdfs:comment """This property links a PublicService with the rules that it follow.

Unline cpsv:follow whose range is a Rule, the range of this property is simply an xsd:string."""@en ;
      rdfs:domain esproc:Procedimiento ;
      rdfs:range xsd:string .

esproc:detalleTramitacionTelefonoTexto
      a       owl:DatatypeProperty ;
      rdfs:comment "This property links a telefone-based PublicService with the rules that it follows (in text format)."@en ;
      rdfs:domain esproc:ProcedimientoPorTelefono ;
      rdfs:range xsd:string ;
      rdfs:subPropertyOf esproc:followsTexto .

esproc:CentroServicio
      a       owl:Class ;
      rdfs:comment "a subclass of org:Organization, the class CentroServicio represent organizations that are involved in the Public Service activities."@en ;
      rdfs:subClassOf <http://www.w3.org/ns/org#Organization> .

esproc:impreso
      a       owl:ObjectProperty ;
      rdfs:comment "This property links a Public Service with its applications forms."@en ;
      rdfs:domain esproc:Procedimiento ;
      rdfs:range esproc:Impreso ;
      rdfs:subPropertyOf <http://purl.org/vocab/cpsv#hasInput> .

esproc:Recurso
      a       owl:Class ;
      rdfs:comment "To  be completed"@en .

<http://purl.org/vocab/cpsv#uses>
      owl:inverseOf esproc:usadoPor .

<http://www.geonames.org/ontology#R.ST>
      a       owl:NamedIndividual , skos:Concept .

esproc:realizacion
      a       owl:ObjectProperty ;
      rdfs:comment "This property links a PublicService with the places/organization in which the service is realized."@en ;
      rdfs:domain esproc:Procedimiento ;
      rdfs:range esproc:CentroServicio ;
      rdfs:subPropertyOf <http://purl.org/vocab/cpsv#hasChannel> .

<http://purl.org/vocab/cpsv#physicallyAvailableAt>
      rdfs:subPropertyOf <http://purl.org/vocab/cpsv#hasChannel> .

esproc:destino
      a       owl:ObjectProperty ;
      rdfs:comment "This property links a Public Service to an organization in which the Public Service should be addressed to."@en ;
      rdfs:domain esproc:Procedimiento ;
      rdfs:range esproc:CentroServicio ;
      rdfs:subPropertyOf <http://purl.org/vocab/cpsv#hasChannel> .
